software-foundations/programming-language-foundations/OperationalSemantics/general.v
@@ -1,0 +1,35 @@
+Require Import Utf8.
+Require Import Relations.
+
+Definition deterministic {X : Type} (R : relation X) :=
+  ∀ x y1 y2 : X, R x y1 → R x y2 → y1 = y2.
+
+Definition normal_form {X : Type} (R : relation X) (t : X) : Prop :=
+  ¬ ∃ t', R t t'.
+
+Inductive multi {X : Type} (R : relation X) : relation X :=
+| multi_refl : ∀ (x : X), multi R x x
+| multi_step : ∀ (x y z : X), R x y → multi R y z → multi R x z.
+
+
+Theorem multi_R : ∀ {X : Type} (R : relation X) (x y : X),
+  R x y → multi R x y.
+Proof.
+  intros X R x y Rxy.
+  apply multi_step with y.
+  - assumption.
+  - constructor.
+Qed.
+
+Theorem multi_trans : ∀ {X : Type} (R : relation X) (x y z : X),
+  multi R x y → multi R y z → multi R x z.
+Proof.
+  intros X R x y z Rxy Ryz.
+  induction Rxy.
+  - assumption.
+  - eapply multi_step; eauto.
+Qed.
+
+Definition normalizing {X : Type} (R : relation X) :=
+  ∀ t, ∃ t', multi R t t' ∧ normal_form R t'.
+
